C-verifier/src/Midend-IVL/Isabelle-UTP-Extended/theories/Design/utp_designs_more.thy
@@ -29,8 +29,8 @@ section {*Type projections and injections*}
 subsection {*Substitution lift and drop*}
 
 abbreviation lift_rel_usubst_des ("\<lceil>_\<rceil>\<^sub>S\<^sub>D")
-where "\<lceil>\<sigma>\<rceil>\<^sub>S\<^sub>D \<equiv> \<sigma> \<oplus>\<^sub>s (\<Sigma>\<^sub>D \<times>\<^sub>L \<Sigma>\<^sub>D)"
-
+  where "\<lceil>\<sigma>\<rceil>\<^sub>S\<^sub>D \<equiv> \<sigma> \<oplus>\<^sub>s (\<Sigma>\<^sub>D \<times>\<^sub>L \<Sigma>\<^sub>D)"
+    
 abbreviation lift_usubst_des ("\<lceil>_\<rceil>\<^sub>s\<^sub>D")
 where "\<lceil>\<sigma>\<rceil>\<^sub>s\<^sub>D \<equiv> \<lceil>\<lceil>\<sigma>\<rceil>\<^sub>s\<rceil>\<^sub>S\<^sub>D"
 
